Gates.v
@@ -7,14 +7,16 @@ Definition ZX_H :=
     (Z_Spider 1 1 (PI/2)) ⟷ (X_Spider 1 1 (PI/2)) ⟷ (Z_Spider 1 1 (PI/2)).
 Global Opaque ZX_H.
 
-Notation nH := (fun n => nStack1 n ZX_H).
+Notation "□" := (ZX_H). (* \square*)
+
+Notation nH := (fun n => n ↑ □).
 
 Definition ZX_CNOT_l : ZX 2 2 :=  
-        ((Z_Spider 1 2 0%R) ↕ Wire) ⟷ (Wire ↕ (X_Spider 2 1 0%R)).
+        ((Z_Spider 1 2 0%R) ↕ —) ⟷ (— ↕ (X_Spider 2 1 0%R)).
 Global Opaque ZX_CNOT_l.
 
 Definition ZX_CNOT_r : ZX 2 2 := 
-    (Wire ↕ (X_Spider 1 2 0%R)) ⟷ ((Z_Spider 2 1 0%R) ↕ Wire).
+    (— ↕ (X_Spider 1 2 0%R)) ⟷ ((Z_Spider 2 1 0%R) ↕ —).
 Global Opaque ZX_CNOT_r.
 
 Definition ZX_S : ZX 1 1 := Z_Spider 1 1 (PI / 2).
@@ -30,10 +32,12 @@ Notation ZX_CNOT := ZX_CNOT_l.
 Global Opaque ZX_CNOT.
 
 Definition ZX_FLIPPED_CNOT := 
-    (Wire ↕ (Z_Spider 1 2 0%R)) ⟷ ((X_Spider 2 1 0%R) ↕ Wire).
+    (— ↕ (Z_Spider 1 2 0%R)) ⟷ ((X_Spider 2 1 0%R) ↕ —).
    
 Definition ZX_SWAP : ZX 2 2 :=
     ZX_CNOT ⟷ ZX_FLIPPED_CNOT ⟷ ZX_CNOT.
 Global Opaque ZX_SWAP.
+
+Notation "⨉" := ZX_SWAP.
 
 Local Close Scope ZX_scope.
